new/should_build.v
@@ -9,6 +9,8 @@ From New.proof.github_com.goose_lang.goose.testdata.examples
 (* TODO: change to importing the proof once that works *)
 From New.generatedproof.github_com.goose_lang.goose.testdata.examples
   Require channel.
+From New.proof.github_com.mit_pdos.tulip
+  Require program_prelude.
 
 From New.proof Require go_etcd_io.etcd.client.v3.leasing.
 From New.proof Require Import chan context.
